Faster proof for arm/proofs/bignum_k{mul,sqr}_*_neon.ml
This makes the proofs of `arm/proofs/bignum_k{mul,sqr}_{16_32,32_64}_neon.ml`
faster by unusing the inlined hoare triple proofs for local 8->16 multiplication
and instead using the corresponding lemmas in bignum_{mul,sqr}_8_16_neon.ml.

arm/proofs/bignum_mul_8_16_neon.ml
@@ -562,7 +562,7 @@ let bignum_mul_8_16_equiv_output_states = new_definition
 let equiv_goal = mk_equiv_statement
   `ALL (nonoverlapping (z,8 * 16)) [
       (word pc:int64,LENGTH bignum_mul_8_16_mc);
-      (word pc2:int64,LENGTH bignum_mul_8_16_neon_mc);
+      (word pc2:int64,LENGTH bignum_mul_8_16_neon_core_mc);
       (x,8 * 8); (y,8 * 8)]`
   bignum_mul_8_16_equiv_input_states
   bignum_mul_8_16_equiv_output_states
@@ -572,7 +572,7 @@ let equiv_goal = mk_equiv_statement
                         X17; X19; X20; X21; X22; X23; X24] ,,
             MAYCHANGE [memory :> bytes(z,8 * 16)] ,,
             MAYCHANGE SOME_FLAGS`
-  bignum_mul_8_16_neon_core_mc 12
+  bignum_mul_8_16_neon_core_mc 0
   `MAYCHANGE [PC; X1; X2; X3; X4; X5; X6; X7; X8;
                         X9; X10; X11; X12; X13; X14; X15; X16;
                         X17; X19; X20; X21; X22; X23; X24] ,,
@@ -610,7 +610,8 @@ let BIGNUM_MUL_8_16_EQUIV = prove(
   equiv_goal,
 
   REWRITE_TAC[SOME_FLAGS;ALL;NONOVERLAPPING_CLAUSES;BIGNUM_MUL_8_16_EXEC;
-              BIGNUM_MUL_8_16_NEON_EXEC;BIGNUM_MUL_8_16_CORE_EXEC] THEN
+              BIGNUM_MUL_8_16_NEON_EXEC;BIGNUM_MUL_8_16_CORE_EXEC;
+              BIGNUM_MUL_8_16_NEON_CORE_EXEC] THEN
   REPEAT STRIP_TAC THEN
   (** Initialize **)
   EQUIV_INITIATE_TAC bignum_mul_8_16_equiv_input_states THEN
@@ -625,10 +626,9 @@ let BIGNUM_MUL_8_16_EQUIV = prove(
     BIGNUM_MUL_8_16_CORE_EXEC THEN
   ASSERT_NONOVERLAPPING_MODULO_TAC
     `nonoverlapping_modulo (2 EXP 64)
-        (val (z:int64),8 * 16) (pc2 + 12,LENGTH bignum_mul_8_16_neon_core_mc)`
+        (val (z:int64),8 * 16) (pc2,LENGTH bignum_mul_8_16_neon_core_mc)`
     BIGNUM_MUL_8_16_NEON_CORE_EXEC THEN
   ABBREV_TAC `pc' = pc + 12` THEN
-  ABBREV_TAC `pc2' = pc2 + 12` THEN
 
   (* The main simulation part *)
   EQUIV_STEPS_TAC actions
@@ -641,21 +641,18 @@ let BIGNUM_MUL_8_16_EQUIV = prove(
     (** SUBGOAL 0. PC **)
     EXPAND_TAC "pc'" THEN CONV_TAC WORD_RULE;
 
-    (** SUBGOAL 1. PC2 **)
-    EXPAND_TAC "pc2'" THEN CONV_TAC WORD_RULE;
-
-    (** SUBGOAL 2. Outputs **)
+    (** SUBGOAL 1. Outputs **)
     ASM_REWRITE_TAC[bignum_mul_8_16_equiv_output_states;mk_equiv_regs;mk_equiv_bool_regs;
                     BIGNUM_EXPAND_CONV `bignum_from_memory (ptr,8) state`;
                     C_ARGUMENTS] THEN
     REPEAT (HINT_EXISTS_REFL_TAC THEN ASM_REWRITE_TAC[]) THEN
     ASM_REWRITE_TAC[BIGNUM_EXPAND_CONV `bignum_from_memory (p,16) st`];
 
-    (** SUBGOAL 3. MAYCHANGE left **)
+    (** SUBGOAL 2. MAYCHANGE left **)
     DISCARD_ASSUMPTIONS_TAC (fun th -> free_in `s0':armstate` (concl th)) THEN
     MONOTONE_MAYCHANGE_TAC;
 
-    (** SUBGOAL 4. MAYCHANGE right **)
+    (** SUBGOAL 3. MAYCHANGE right **)
     DISCARD_ASSUMPTIONS_TAC (fun th -> free_in `s0:armstate` (concl th)) THEN
     MONOTONE_MAYCHANGE_TAC
   ]);;
@@ -735,17 +732,17 @@ let BIGNUM_MUL_8_16_CORE_CORRECT_N =
 (** Finally, we prove the correctness of core of bignum_mul_8_16_neon
     using BIGNUM_MUL_8_16_CORE_CORRECT_N and BIGNUM_MUL_8_16_EQUIV!
 **)
-let BIGNUM_MUL_8_16_NEON_CORRECT = prove(
+let BIGNUM_MUL_8_16_NEON_CORE_CORRECT = prove(
   `!z x y a b pc2.
       ALL (nonoverlapping (z,8 * 16))
-          [(word pc2,LENGTH bignum_mul_8_16_neon_mc); (x,8 * 8); (y,8 * 8)]
+          [(word pc2,LENGTH bignum_mul_8_16_neon_core_mc); (x,8 * 8); (y,8 * 8)]
       ==> ensures arm
-            (\s. aligned_bytes_loaded s (word pc2) bignum_mul_8_16_neon_mc /\
-                 read PC s = word(pc2 + 0xc) /\
+            (\s. aligned_bytes_loaded s (word pc2) bignum_mul_8_16_neon_core_mc /\
+                 read PC s = word(pc2) /\
                  C_ARGUMENTS [z; x; y] s /\
                  bignum_from_memory (x,8) s = a /\
                  bignum_from_memory (y,8) s = b)
-          (\s. read PC s = word (pc2 + 1984) /\
+          (\s. read PC s = word (pc2 + LENGTH bignum_mul_8_16_neon_core_mc) /\
                bignum_from_memory (z,16) s = a * b)
             (MAYCHANGE [PC; X1; X2; X3; X4; X5; X6; X7; X8;
                         X9; X10; X11; X12; X13; X14; X15; X16;
@@ -754,8 +751,8 @@ let BIGNUM_MUL_8_16_NEON_CORRECT = prove(
              MAYCHANGE [memory :> bytes(z,8 * 16)] ,,
              MAYCHANGE SOME_FLAGS)`,
 
-  let mc_lengths_th =
-    map (fst o CONJ_PAIR) [BIGNUM_MUL_8_16_EXEC; BIGNUM_MUL_8_16_NEON_EXEC] in
+  (*let mc_lengths_th =
+    map (fst o CONJ_PAIR) [BIGNUM_MUL_8_16_EXEC; BIGNUM_MUL_8_16_NEON_EXEC] in*)
   REPEAT GEN_TAC THEN
 
   (* Prepare pc for the 'left' program. The left program must not have overwritten x and y. *)
@@ -776,10 +773,10 @@ let BIGNUM_MUL_8_16_NEON_CORRECT = prove(
   REPEAT_N 2 STRIP_TAC THEN
 
   VCGEN_EQUIV_TAC BIGNUM_MUL_8_16_EQUIV BIGNUM_MUL_8_16_CORE_CORRECT_N
-    [BIGNUM_MUL_8_16_EXEC; BIGNUM_MUL_8_16_NEON_EXEC] THEN
+    [BIGNUM_MUL_8_16_EXEC; BIGNUM_MUL_8_16_NEON_CORE_EXEC] THEN
 
   (* unravel definitions that may block reasonings *)
-  RULE_ASSUM_TAC (REWRITE_RULE([ALL;NONOVERLAPPING_CLAUSES] @ mc_lengths_th)) THEN
+  RULE_ASSUM_TAC (REWRITE_RULE([ALL;NONOVERLAPPING_CLAUSES;BIGNUM_MUL_8_16_EXEC])) THEN
   REPEAT SPLIT_FIRST_CONJ_ASSUM_TAC THEN
   REWRITE_TAC[C_ARGUMENTS;BIGNUM_FROM_MEMORY_BYTES] THEN
   REPEAT CONJ_TAC THENL [
@@ -795,13 +792,13 @@ let BIGNUM_MUL_8_16_NEON_CORRECT = prove(
           (word (pc+12),LENGTH (APPEND bignum_mul_8_16_core_mc barrier_inst_bytes)))
           (APPEND bignum_mul_8_16_core_mc barrier_inst_bytes)
           (write PC (word (pc+12)) s2)` THEN
-    SUBGOAL_THEN `aligned_bytes_loaded s2 (word (pc2 + 12):int64) bignum_mul_8_16_neon_core_mc`
+    (*SUBGOAL_THEN `aligned_bytes_loaded s2 (word (pc2 + 12):int64) bignum_mul_8_16_neon_core_mc`
       (fun th -> REWRITE_TAC[th]) THENL [
       REWRITE_TAC[bignum_mul_8_16_neon_core_mc_def] THEN
       IMP_REWRITE_TAC[WORD_ADD;ALIGNED_BYTES_LOADED_SUB_LIST] THEN
       CONV_TAC NUM_DIVIDES_CONV THEN NO_TAC;
       ALL_TAC
-    ] THEN
+    ] THEN*)
     SUBGOAL_THEN `4 divides val (word (pc+12):int64)` ASSUME_TAC THENL [
       IMP_REWRITE_TAC[DIVIDES_4_VAL_WORD_ADD_64] THEN CONV_TAC NUM_DIVIDES_CONV;
       ALL_TAC
@@ -813,9 +810,52 @@ let BIGNUM_MUL_8_16_NEON_CORRECT = prove(
     PROVE_CONJ_OF_EQ_READS_TAC BIGNUM_MUL_8_16_CORE_EXEC;
 
     (** SUBGOAL 2. Postcond **)
-    MESON_TAC[bignum_mul_8_16_equiv_output_states;BIGNUM_FROM_MEMORY_BYTES];
+    MESON_TAC[BIGNUM_MUL_8_16_NEON_CORE_EXEC;bignum_mul_8_16_equiv_output_states;BIGNUM_FROM_MEMORY_BYTES];
 
     (** SUBGOAL 3. Frame **)
+    MESON_TAC[]
+  ]);;
+
+let BIGNUM_MUL_8_16_NEON_CORRECT = prove(
+  `!z x y a b pc2.
+      ALL (nonoverlapping (z,8 * 16))
+          [(word pc2,LENGTH bignum_mul_8_16_neon_mc); (x,8 * 8); (y,8 * 8)]
+      ==> ensures arm
+            (\s. aligned_bytes_loaded s (word pc2) bignum_mul_8_16_neon_mc /\
+                 read PC s = word(pc2 + 0xc) /\
+                 C_ARGUMENTS [z; x; y] s /\
+                 bignum_from_memory (x,8) s = a /\
+                 bignum_from_memory (y,8) s = b)
+          (\s. read PC s = word (pc2 + 1984) /\
+               bignum_from_memory (z,16) s = a * b)
+            (MAYCHANGE [PC; X1; X2; X3; X4; X5; X6; X7; X8;
+                        X9; X10; X11; X12; X13; X14; X15; X16;
+                        X17; X19; X20; X21; X22; X23; X24] ,,
+             MAYCHANGE [Q0; Q1; Q2; Q3; Q4; Q5],,
+             MAYCHANGE [memory :> bytes(z,8 * 16)] ,,
+             MAYCHANGE SOME_FLAGS)`,
+
+  REPEAT GEN_TAC THEN
+  DISCH_THEN (ASSUME_TAC o (REWRITE_RULE [BIGNUM_MUL_8_16_NEON_EXEC])) THEN
+  MP_TAC (SPECL [`z:int64`;`x:int64`;`y:int64`;`a:num`;`b:num`;`pc2+12`]
+    (REWRITE_RULE[BIGNUM_MUL_8_16_NEON_CORE_EXEC]
+       BIGNUM_MUL_8_16_NEON_CORE_CORRECT)) THEN
+  ANTS_TAC THENL [
+    FIRST_X_ASSUM MP_TAC THEN
+    REWRITE_TAC[ALL; NONOVERLAPPING_CLAUSES] THEN
+    STRIP_TAC THEN REPEAT CONJ_TAC THEN NONOVERLAPPING_TAC;
+    ALL_TAC
+  ] THEN
+  MATCH_MP_TAC ENSURES_SUBLEMMA_THM THEN REWRITE_TAC[] THEN
+  REPEAT CONJ_TAC THENL [
+    REPEAT STRIP_TAC THEN ASM_REWRITE_TAC[bignum_mul_8_16_neon_core_mc_def] THEN
+    REWRITE_TAC[WORD_RULE`word (pc2+12):int64 = word_add (word pc2) (word 12)`] THEN
+    IMP_REWRITE_TAC[ALIGNED_BYTES_LOADED_SUB_LIST] THEN
+    CONV_TAC NUM_DIVIDES_CONV;
+
+    SUBSUMED_MAYCHANGE_TAC;
+
+    REWRITE_TAC[GSYM ADD_ASSOC] THEN CONV_TAC (ONCE_DEPTH_CONV NUM_ADD_CONV) THEN
     MESON_TAC[]
   ]);;
 
